\section{Substitution}

\begin{center}
\begin{align*}
y' &= f(ax+by+c) \\
&\Downarrow \\
u &= u(x) = ax +by +c\\
\frac{du}{dx} &= a + b\frac{dy}{dx}\\
\frac{du}{dx} &= a +b\cdot u\\
\frac{du}{a+b\cdot u} &= dx\\
&\Downarrow \text{Variablentrennung}\\
y &= \frac{u-a-c}{b}
\end{align*}
\end{center}

\begin{center}
\begin{align*}
y' &= f\left(\frac{y}{x}\right)\Rightarrow u =\frac{y}{x}\\
y &= u\cdot x\\
y' &= u'\cdot x + u \Rightarrow f(u) = u'\cdot x +u\\
\frac{du}{dx} &= \frac{f(u)-u}{x}\\
&\Downarrow \text{Variablentrennung}\\
u &= u(x) \Rightarrow u = \frac{y}{x}\\
y &= u(x)\cdot x
\end{align*}
\end{center}
